TseitinProofs.fst
@@ -12,27 +12,57 @@ open TseitinCore
 
 
 
-let rec append_valid_cnf_formulas (f1 : list (list int)) (f2 : list (list int))
-    : Lemma (requires valid_cnf_formula f1 /\ valid_cnf_formula f2)
-            (ensures valid_cnf_formula (f1 @ f2))
-    = if L.length f1 = 0 then ()
-      else append_valid_cnf_formulas (tl f1) f2
+// let rec append_valid_cnf_formulas (f1 : list (list int)) (f2 : list (list int))
+//     : Lemma (requires valid_cnf_formula f1 /\ valid_cnf_formula f2)
+//             (ensures valid_cnf_formula (f1 @ f2))
+//     = if L.length f1 = 0 then ()
+//       else append_valid_cnf_formulas (tl f1) f2
 
 
-let rec append_variables_in_interval (f1 : list (list int)) (f2 : list (list int))
-                                     (n:nat) (start_interval:nat) (end_interval:nat)
-    : Lemma (requires n <= start_interval /\ start_interval <= end_interval /\
-                      valid_cnf_formula f1 /\ valid_cnf_formula f2 /\
-                      variables_in_interval f1 n start_interval end_interval /\
-                      variables_in_interval f2 n start_interval end_interval)
-            (ensures valid_cnf_formula (f1 @ f2) /\ variables_in_interval (f1 @ f2) n start_interval end_interval)
-    = append_valid_cnf_formulas f1 f2;
-      if f1 = [] then ()
-      else 
-      (
-          append_valid_cnf_formulas (L.tl f1) f2;
-          append_variables_in_interval (tl f1) f2 n start_interval end_interval
-      )
+// let rec append_variables_in_interval (f1 : list (list int)) (f2 : list (list int))
+//                                      (n:nat) (start_interval:nat) (end_interval:nat)
+//     : Lemma (requires n <= start_interval /\ start_interval <= end_interval /\
+//                       valid_cnf_formula f1 /\ valid_cnf_formula f2 /\
+//                       variables_in_interval f1 n start_interval end_interval /\
+//                       variables_in_interval f2 n start_interval end_interval)
+//             (ensures valid_cnf_formula (f1 @ f2) /\ variables_in_interval (f1 @ f2) n start_interval end_interval)
+//     = append_valid_cnf_formulas f1 f2;
+//       if f1 = [] then ()
+//       else 
+//       (
+//           append_valid_cnf_formulas (L.tl f1) f2;
+//           append_variables_in_interval (tl f1) f2 n start_interval end_interval
+//       )
+
+
+let not_clauses_in_interval (v1:int) (v:int) (n:nat) (start_interval:nat) (end_interval:nat)
+    : Lemma (requires n <= start_interval /\ start_interval <= v &&
+                      valid_variable v1 && valid_variable v &&
+                      variable_in_interval v1 n start_interval v &&
+                      end_interval = v + 1)
+            (ensures variables_in_interval (not_clauses v1 v) n start_interval end_interval)
+    = ()
+
+
+// let aux (tau : list bool) 
+//         (f1:formula_t) (rf1 : list (list int)) (v1:int) (n:nat)
+//         (start_interval:nat) (end_interval:nat) (rf : list (list int)) (v:int)
+//     : Lemma (requires n <= start_interval /\ start_interval <= v /\
+//                       valid f1 rf1 v1 n start_interval v /\
+//                       tseitin_same_value f1 rf1 v1 n start_interval v /\
+//                       rf = rf1 @ (not_clauses v1 v) /\
+//                       end_interval = v + 1 /\
+//                       valid_cnf_formula rf /\
+//                       L.length tau >= end_interval /\
+//                       variables_up_to_cnf_formula rf (L.length tau) /\
+//                       truth_value_cnf_formula rf tau)
+//             (ensures variables_up_to (Not f1) (L.length tau) &&
+//                      variables_up_to_literal (pos_var_to_lit v) (L.length tau) &&
+//                      truth_value_literal (pos_var_to_lit v) tau = truth_value (Not f1) tau)
+//     = variables_up_to_monotone f1 n (L.length tau);
+//       assert (truth_value_literal (pos_var_to_lit v1) tau = truth_value f1 tau);
+//       lemma_not_clauses v1 v tau;
+//       assert (truth_value_literal (pos_var_to_lit v) tau = truth_value (Not f1) tau)
 
 
 let prove_same_value_not (f1:formula_t) (rf1 : list (list int)) (v1:int) (n:nat)
@@ -45,41 +75,24 @@ let prove_same_value_not (f1:formula_t) (rf1 : list (list int)) (v1:int) (n:nat)
             (ensures valid (Not f1) rf v n start_interval end_interval /\
                      tseitin_same_value (Not f1) rf v n start_interval end_interval)
     = append_valid_cnf_formulas rf1 (not_clauses v1 v);
-
       variables_in_interval_monotone rf1 n start_interval v end_interval;
-      assert (variables_in_interval rf1 n start_interval end_interval);
-
-      let nc = not_clauses v1 v in
-      assert (variables_in_interval_literal (L.index (L.index nc 0) 0) n start_interval end_interval);
-      assert (variables_in_interval_literal (L.index (L.index nc 0) 1) n start_interval end_interval);
-      assert (variables_in_interval_literal (L.index (L.index nc 1) 0) n start_interval end_interval);
-      assert (variables_in_interval_literal (L.index (L.index nc 1) 1) n start_interval end_interval);
-      // assert (L.index nc 0 = [L.index (L.index nc 0) 0; L.index (L.index nc 0) 1]);
-      assert (L.index nc 0 = [L.index (L.index nc 0) 0; L.index (L.index nc 0) 1] &&
-              variables_in_interval_literal (L.index (L.index nc 0) 0) n start_interval end_interval &&
-              variables_in_interval_literal (L.index (L.index nc 0) 1) n start_interval end_interval ==>
-              variables_in_interval_clause (L.index nc 0) n start_interval end_interval);
-      // assert (variables_in_interval_clause (L.index nc 0) n start_interval end_interval);
-      assert (L.index nc 1 = [L.index (L.index nc 1) 0; L.index (L.index nc 1) 1]);
-      assert (variables_in_interval_clause (L.index nc 1) n start_interval end_interval);
-      assert (variables_in_interval nc n start_interval end_interval);
-
-      assert (variables_in_interval (not_clauses v1 v) n start_interval end_interval);
-
+      not_clauses_in_interval v1 v n start_interval end_interval;
       append_variables_in_interval rf1 (not_clauses v1 v) n start_interval end_interval;
-      assert (variables_in_interval rf n start_interval end_interval);
       assert (valid (Not f1) rf v n start_interval end_interval);
 
       let aux (tau : list bool) 
           : Lemma (requires L.length tau >= end_interval /\
                             truth_value_cnf_formula rf tau)
-                  (ensures truth_value_literal (pos_var_to_lit v) tau = truth_value (Not f1) tau)
+                  (ensures variables_up_to (Not f1) (L.length tau) &&
+                           variables_up_to_literal (pos_var_to_lit v) (L.length tau) &&
+                           truth_value_literal (pos_var_to_lit v) tau = truth_value (Not f1) tau)
           = variables_up_to_monotone f1 n (L.length tau);
             assert (truth_value_literal (pos_var_to_lit v1) tau = truth_value f1 tau);
             lemma_not_clauses v1 v tau;
             assert (truth_value_literal (pos_var_to_lit v) tau = truth_value (Not f1) tau)
       in
       forall_intro (move_requires aux)
+
 
 
 // let prove_same_value_or (f1:formula_t) (rf1 : list (list int)) (v1:int)
@@ -228,27 +241,32 @@ let prove_same_value_not (f1:formula_t) (rf1 : list (list int)) (v1:int) (n:nat)
 //                       end_interval = v + 1)
 //             (ensures valid (Not f1) rf v n start_interval end_interval /\
 //                      tseitin_can_extend (Not f1) rf v n start_interval end_interval)
-//     = assert (valid (Not f1) rf v n start_interval end_interval);
+//     = append_valid_cnf_formulas rf1 (not_clauses v1 v);
+//       variables_in_interval_monotone rf1 n start_interval v end_interval;
+//       not_clauses_in_interval v1 v n start_interval end_interval;
+//       append_variables_in_interval rf1 (not_clauses v1 v) n start_interval end_interval;
+//       assert (valid (Not f1) rf v n start_interval end_interval);
+
 //       let aux (tau : list bool) 
 //           : Lemma (requires L.length tau = n)
-//                   (ensures can_extend tau (Not f1) rf v n start_interval end_interval)
+//                   (ensures L.length tau = n /\
+//                            can_extend tau (Not f1) rf v n start_interval end_interval)
 //           = assert (can_extend tau f1 rf1 v1 n start_interval v);
 //             assert (valid_literal (pos_var_to_lit v1));
             
 //             let conditions (tau1 : list bool) =
-//                 // tau <= tau1 /\
-//                 L.length tau1 = v /\
-//                 truth_value_cnf_formula rf1 tau1 /\
+//                 is_prefix tau tau1 &&
+//                 L.length tau1 = v &&
+//                 truth_value_cnf_formula rf1 tau1 &&
 //                 truth_value f1 tau = truth_value_literal (pos_var_to_lit v1) tau1
 //             in
-//             let extract_from_exists : (tau1 : list bool {conditions tau1}) -> prop = fun (tau1 : list bool) -> conditions tau1 in
-//             let tau1 : list bool = FStar.IndefiniteDescription.indefinite_description_ghost (list bool) extract_from_exists in
+//             assume (exists x . conditions x);
+//             let tau1 = extract_value conditions in
 
 //             negate_literal v1 tau1;
 
 //             let tau' = combine1 tau tau1 n start_interval v (truth_value (Not f1) tau) in
-//             // assert (tau <= tau');
-//             assert (L.length tau' = end_interval);
+//             is_prefix_then_is_interval tau tau1;
 //             transfer_truth_value rf1 tau1 tau' n start_interval v;
 
 //             transfer_truth_value_lit (pos_var_to_lit v1) tau1 tau' n start_interval v;
@@ -256,8 +274,7 @@ let prove_same_value_not (f1:formula_t) (rf1 : list (list int)) (v1:int) (n:nat)
 //             transfer_truth_value_lit (neg_var_to_lit v1) tau1 tau' n start_interval v;
 //             assert (truth_value_literal (neg_var_to_lit v1) tau1 = not (truth_value_literal (pos_var_to_lit v1) tau1));
 
-//             lemma_not_clauses v1 v tau';
-//             assert (truth_value_cnf_formula rf tau')
+//             lemma_not_clauses v1 v tau'
 //       in
 //       forall_intro (move_requires aux) 
 
